src/impl/TLS13.Impl.Handle.Handshake.fst
@@ -14,12 +14,16 @@ module M = TLS13.Messages
 module Seq = FStar.Seq
 module SZ = FStar.SizeT
 module U8 = FStar.UInt8
+module WS = TLS13.Wire.Spec
 
-fn handle_handshake_message
+fn handle_unexpected_handshake_input
   (c:C.connection_state)
+  (content_type:U8.t)
   (l:L.tls_message)
   (raw:array U8.t)
   (raw_len:SZ.t)
+  (fragment:array U8.t)
+  (fragment_len:SZ.t)
   (network_out:array U8.t)
   (network_out_len:SZ.t)
   (app_out:array U8.t)
@@ -27,23 +31,31 @@ fn handle_handshake_message
   requires C.connection_exactly c 'st0 **
            (exists* m. L.is_valid_tls_message l m) **
            pts_to raw 'raw_bytes **
+           pts_to fragment 'fragment_bytes **
            pts_to network_out 'old_network_out **
            pts_to app_out 'old_app_out **
            pure (B.length 'raw_bytes == SZ.v raw_len /\
+                 B.length 'fragment_bytes == SZ.v fragment_len /\
                  B.length 'old_network_out == SZ.v network_out_len /\
-           B.length 'old_app_out == SZ.v app_out_len /\
-           L.tls_message_is_handshake l)
+                 B.length 'old_app_out == SZ.v app_out_len /\
+                 (exists ct msg.
+                   L.content_type_matches content_type ct /\
+                   WS.parse_tls_message ct (Ghost.reveal 'fragment_bytes) == Some msg))
   returns resp: CT.client_response
   ensures C.connection_exactly c (C.local_fail_state 'st0 C.tls_unexpected_message_error) **
           pts_to raw 'raw_bytes **
+          pts_to fragment 'fragment_bytes **
           pts_to network_out 'old_network_out **
           pts_to app_out 'old_app_out **
           pure (B.length 'old_network_out == SZ.v network_out_len /\
                 B.length 'old_app_out == SZ.v app_out_len /\
-                CT.unexpected_message_response
+                CT.legal_network_response
                   'st0
                   (C.local_fail_state 'st0 C.tls_unexpected_message_error)
                   resp
+                  content_type
+                  (Ghost.reveal 'fragment_bytes)
+                  (Ghost.reveal 'raw_bytes)
                   'old_network_out
                   'old_app_out /\
                 CT.some_legal_response
@@ -70,6 +82,15 @@ fn handle_handshake_message
     resp
     'old_network_out
     'old_app_out));
+  CT.lemma_legal_network_response_unexpected_from_parse_success
+    'st0
+    (C.local_fail_state 'st0 C.tls_unexpected_message_error)
+    resp
+    content_type
+    (Ghost.reveal 'fragment_bytes)
+    (Ghost.reveal 'raw_bytes)
+    'old_network_out
+    'old_app_out;
   assert (pure (CT.some_legal_response
     'st0
     (C.local_fail_state 'st0 C.tls_unexpected_message_error)
@@ -77,4 +98,275 @@ fn handle_handshake_message
     'old_network_out
     'old_app_out));
   resp
+}
+
+fn handle_handshake_message
+  (c:C.connection_state)
+  (content_type:U8.t)
+  (l:L.tls_message)
+  (raw:array U8.t)
+  (raw_len:SZ.t)
+  (fragment:array U8.t)
+  (fragment_len:SZ.t)
+  (network_out:array U8.t)
+  (network_out_len:SZ.t)
+  (app_out:array U8.t)
+  (app_out_len:SZ.t)
+  requires C.connection_exactly c 'st0 **
+           (exists* m. L.is_valid_tls_message l m) **
+           pts_to raw 'raw_bytes **
+           pts_to fragment 'fragment_bytes **
+           pts_to network_out 'old_network_out **
+           pts_to app_out 'old_app_out **
+           pure (B.length 'raw_bytes == SZ.v raw_len /\
+                 B.length 'fragment_bytes == SZ.v fragment_len /\
+                 B.length 'old_network_out == SZ.v network_out_len /\
+                 B.length 'old_app_out == SZ.v app_out_len /\
+                 L.tls_message_is_handshake l /\
+                 (exists ct msg.
+                   L.content_type_matches content_type ct /\
+                   WS.parse_tls_message ct (Ghost.reveal 'fragment_bytes) == Some msg) /\
+                 CT.network_input_wf
+                   'st0
+                   content_type
+                   (Ghost.reveal 'fragment_bytes)
+                   (Ghost.reveal 'raw_bytes) /\
+                 CT.parsed_message_wire_success
+                   content_type
+                   (Ghost.reveal 'fragment_bytes)
+                   l)
+  returns resp: CT.client_response
+  ensures exists* st1.
+          C.connection_exactly c st1 **
+          pts_to raw 'raw_bytes **
+          pts_to fragment 'fragment_bytes **
+          pts_to network_out 'old_network_out **
+          pts_to app_out 'old_app_out **
+          pure (B.length 'old_network_out == SZ.v network_out_len /\
+                B.length 'old_app_out == SZ.v app_out_len /\
+                CT.legal_network_response
+                  'st0
+                  st1
+                  resp
+                  content_type
+                  (Ghost.reveal 'fragment_bytes)
+                  (Ghost.reveal 'raw_bytes)
+                  'old_network_out
+                  'old_app_out /\
+                CT.some_legal_response
+                  'st0
+                  st1
+                  resp
+                  'old_network_out
+                  'old_app_out)
+{
+  match l {
+    L.LTlsHandshake lhs -> {
+      match lhs {
+        L.LHelloRetryRequest -> {
+          assert (pure (CT.parsed_message_wire_success
+            content_type
+            (Ghost.reveal 'fragment_bytes)
+            (L.LTlsHandshake L.LHelloRetryRequest)));
+          assert (pure (CT.wire_parse_success
+            content_type
+            (Ghost.reveal 'fragment_bytes)
+            (M.TlsHandshake M.HelloRetryRequest)));
+          assert (pure (CT.received_tls_raw_delta_legal
+            'st0
+            (M.TlsHandshake M.HelloRetryRequest)
+            (Ghost.reveal 'raw_bytes)));
+
+          let waiting = C.is_waiting_server_hello c;
+          if waiting {
+            L.free_tls_message (L.LTlsHandshake L.LHelloRetryRequest);
+            C.mark_received_hello_retry_request_rejected c raw;
+            let resp = {
+              CT.network_out_len = 0sz;
+              CT.app_out_len = 0sz;
+              CT.status = CT.ConnectionFailed;
+            };
+            Seq.lemma_len_slice 'old_network_out 0 0;
+            Seq.lemma_eq_intro B.empty (Seq.slice 'old_network_out 0 0);
+            assert (pure (Seq.equal B.empty (CT.response_network_out resp 'old_network_out)));
+            C.lemma_received_hello_retry_request_rejected_state_evolves
+              'st0
+              (Ghost.reveal 'raw_bytes);
+            assert (pure (CT.legal_received_tls_response
+              'st0
+              (C.received_hello_retry_request_rejected_state 'st0 (Ghost.reveal 'raw_bytes))
+              resp
+              (M.TlsHandshake M.HelloRetryRequest)
+              (Ghost.reveal 'raw_bytes)
+              'old_network_out
+              'old_app_out));
+            assert (pure (CT.legal_handled_tls_response
+              'st0
+              (C.received_hello_retry_request_rejected_state 'st0 (Ghost.reveal 'raw_bytes))
+              resp
+              (M.TlsHandshake M.HelloRetryRequest)
+              (Ghost.reveal 'raw_bytes)
+              'old_network_out
+              'old_app_out));
+            CT.lemma_legal_network_response_handled_from_parse_success
+              'st0
+              (C.received_hello_retry_request_rejected_state 'st0 (Ghost.reveal 'raw_bytes))
+              resp
+              content_type
+              (Ghost.reveal 'fragment_bytes)
+              (M.TlsHandshake M.HelloRetryRequest)
+              (Ghost.reveal 'raw_bytes)
+              'old_network_out
+              'old_app_out;
+            assert (pure (CT.some_legal_response
+              'st0
+              (C.received_hello_retry_request_rejected_state 'st0 (Ghost.reveal 'raw_bytes))
+              resp
+              'old_network_out
+              'old_app_out));
+            resp
+          } else {
+            handle_unexpected_handshake_input
+              c
+              content_type
+              (L.LTlsHandshake L.LHelloRetryRequest)
+              raw
+              raw_len
+              fragment
+              fragment_len
+              network_out
+              network_out_len
+              app_out
+              app_out_len
+          }
+        }
+        L.LClientHello lch -> {
+          handle_unexpected_handshake_input
+            c
+            content_type
+            (L.LTlsHandshake (L.LClientHello lch))
+            raw
+            raw_len
+            fragment
+            fragment_len
+            network_out
+            network_out_len
+            app_out
+            app_out_len
+        }
+        L.LServerHello lsh -> {
+          handle_unexpected_handshake_input
+            c
+            content_type
+            (L.LTlsHandshake (L.LServerHello lsh))
+            raw
+            raw_len
+            fragment
+            fragment_len
+            network_out
+            network_out_len
+            app_out
+            app_out_len
+        }
+        L.LEncryptedExtensions lee -> {
+          handle_unexpected_handshake_input
+            c
+            content_type
+            (L.LTlsHandshake (L.LEncryptedExtensions lee))
+            raw
+            raw_len
+            fragment
+            fragment_len
+            network_out
+            network_out_len
+            app_out
+            app_out_len
+        }
+        L.LCertificate lcert -> {
+          handle_unexpected_handshake_input
+            c
+            content_type
+            (L.LTlsHandshake (L.LCertificate lcert))
+            raw
+            raw_len
+            fragment
+            fragment_len
+            network_out
+            network_out_len
+            app_out
+            app_out_len
+        }
+        L.LCertificateVerify lcv -> {
+          handle_unexpected_handshake_input
+            c
+            content_type
+            (L.LTlsHandshake (L.LCertificateVerify lcv))
+            raw
+            raw_len
+            fragment
+            fragment_len
+            network_out
+            network_out_len
+            app_out
+            app_out_len
+        }
+        L.LFinished lfin -> {
+          handle_unexpected_handshake_input
+            c
+            content_type
+            (L.LTlsHandshake (L.LFinished lfin))
+            raw
+            raw_len
+            fragment
+            fragment_len
+            network_out
+            network_out_len
+            app_out
+            app_out_len
+        }
+      }
+    }
+    L.LTlsApplicationData lapp -> {
+      handle_unexpected_handshake_input
+        c
+        content_type
+        (L.LTlsApplicationData lapp)
+        raw
+        raw_len
+        fragment
+        fragment_len
+        network_out
+        network_out_len
+        app_out
+        app_out_len
+    }
+    L.LTlsAlert lalert -> {
+      handle_unexpected_handshake_input
+        c
+        content_type
+        (L.LTlsAlert lalert)
+        raw
+        raw_len
+        fragment
+        fragment_len
+        network_out
+        network_out_len
+        app_out
+        app_out_len
+    }
+    L.LTlsChangeCipherSpec -> {
+      handle_unexpected_handshake_input
+        c
+        content_type
+        L.LTlsChangeCipherSpec
+        raw
+        raw_len
+        fragment
+        fragment_len
+        network_out
+        network_out_len
+        app_out
+        app_out_len
+    }
+  }
 }
